---
type: post
title: A collection of images and working
---

## Math lessons v1

ALL WRONG...

$$3x^2 + 2x + 3 = 2(x+3)$$



$$\frac{3x^2 + 2x + 3}{2} = x+3$$

$$x = (\frac{3x^2 + 2x + 3}{2}) - 3$$



...$$3x^2 + 2x +3$$

$$\frac{dx}{dy} = x^6 + x^2 + 3$$

$$\frac{dx}{dy} = (3+x)(1+x)$$



$$x = (\frac{(3+x)(1+x)}{2}) - 3$$

$$x = (\frac{3}{2}+\frac{1}{2}+\frac{x}{2}) - 3$$

$$x + 3 = \frac{3}{2}+\frac{1}{2}+\frac{x}{2}$$

$$3 = \frac{3}{2}+\frac{1}{2}+\frac{x}{2} - x$$



$$3 -\frac{3}{2}-\frac{1}{2} \times 2 = x - x$$



```{r}
(3-(3/2)-(1/2))*2
```

$$2 = x - x$$

$$2 \not= x - x$$





## Solutions and Questions...

1. $$3x^2 + 2x + 3 = 2(x+3)$$

