---
layout: post
title:  "dealing with brackets in algebraic equations"
date:   2019-07-17 15:00:56 +1000
categories: math stuff
---
when you have brackets in an algebraic equation and a coeffient attached to it you multiply the coeffiecent by each term in the brackets

E.G. 

$$3(4+x)=12+3x$$

or 

$$n(4+x)=4n+nx$$



if you are multipling 2 sets of brackets together you would take the first term in the first set of brackets and times it with the first term in the second set of brackets. then multiply first term with second term in second brackets. repeat the process with the second term in first brackets.

E.G.

$$(n+2)(n+2)=n*n+2n+2n+4=n^2+4n+4$$



to substract and add brackets together you just have to expand the brackets as necassary then collect all like terms and add or subtract like terms when necassary  

E.G. 

$$3(n-5)+(2+n)= 3n-15+2+n=4n-13$$

or

$$3(n-5)-(2+n)=3n-15-2+n=4n-17$$

